rework tree semantics again

TreeSem.thy
@@ -2,13 +2,20 @@ theory TreeSem
   imports Soundness "HOL-Cardinals.Bounded_Set"
 begin
 
+section \<open> utils \<close>
+
+lemma disjCE:
+  \<open>P \<or> Q \<Longrightarrow> (P \<Longrightarrow> R) \<Longrightarrow> (\<not> P \<Longrightarrow> Q \<Longrightarrow> R) \<Longrightarrow> R\<close>
+  by blast
+
+
 section \<open> Bounded Set Utils \<close>
 
 lemma bmember_bmap_iff:
   \<open>bmember y (map_bset f B) \<longleftrightarrow> (\<exists>x. bmember x B \<and> y = f x)\<close>
   by transfer (force simp add: image_def)
 
-lemma bCollect_eq_bempty_iff:
+lemma bCollect_eq_bempty_iff[simp]:
   \<open>bCollect p = bempty \<longleftrightarrow> (\<nexists>x. p x)\<close>
   by (metis Collect_empty_eq bCollect.rep_eq bempty.rep_eq set_bset_inject)
 
@@ -20,71 +27,75 @@ lemma pred_bCollect_eq[simp]:
   \<open>pred_bset p (bCollect q) = (q \<le> p)\<close>
   by (simp add: bCollect.rep_eq bset.pred_set le_fun_def)
 
+declare bempty.rep_eq[simp]
+declare map_bset.rep_eq[simp]
+declare bCollect.rep_eq[simp]
+
+
 section \<open> Semantic Trees \<close>
 
 datatype 'a label = Env | Local \<open>'a act\<close>
 
 datatype ('c, 's, 'l) sem_tree =
   Branch
-    (config_sem_tree: \<open>'s \<times> 'c\<close>)
+    (comm_sem_tree: 'c)
+    \<comment> \<open> This stores every framed state greater than some base state. \<close>
     (branches_sem_tree:
-      \<open>('l \<times> (('c, 's, 'l) sem_tree + unit)) set[('l \<times> (('s + unit) \<times> 'c)) set]\<close>)
+      \<open>('s \<times> 'l \<times> (('s \<times> ('c, 's, 'l) sem_tree) + unit)) set[('s \<times> 'l \<times> (('s + unit) \<times> 'c)) set]\<close>)
 
 lemma sem_tree_induct:
   \<open>(\<And>ty.
-      (\<And>l tx.
-        (l, Inl tx) \<in> set_bset (branches_sem_tree ty) \<Longrightarrow>
+      (\<And>s l s' tx.
+        (s, l, Inl (s', tx)) \<in> set_bset (branches_sem_tree ty) \<Longrightarrow>
         P tx) \<Longrightarrow>
       P ty) \<Longrightarrow>
     P t\<close>
   apply (rule sem_tree.induct)
   apply (clarsimp simp add: image_def Bex_def)
-  apply (metis sem_tree.sel(2) setl.intros)
+  apply fastforce
   done
 
 function pred_sem_tree
-  :: \<open>('s \<times> 'c \<Rightarrow> bool) \<Rightarrow> ('c, 's, 'l) sem_tree \<Rightarrow> bool\<close>
+  :: \<open>('c \<Rightarrow>
+        ('s \<times> 'l \<times> (('s \<times> ('c, 's, 'l) sem_tree) + unit)) set[('s \<times> 'l \<times> (('s + unit) \<times> 'c)) set] \<Rightarrow>
+        bool) \<Rightarrow>
+      ('c, 's, 'l) sem_tree \<Rightarrow>
+      bool\<close>
   where
-  \<open>pred_sem_tree p (Branch sc S) =
-    (p sc \<and> pred_bset (\<lambda>v. case v of (l,mt') \<Rightarrow> case_sum (pred_sem_tree p) (\<lambda>_. False) mt') S)\<close>
+  \<open>pred_sem_tree p (Branch c S) =
+    (p c S \<and>
+      pred_bset (\<lambda>v. case v of (s,l,mst') \<Rightarrow> case_sum (pred_sem_tree p \<circ> snd) (\<lambda>_. True) mst') S)\<close>
   by pat_completeness auto
 termination
   apply (relation
-      \<open>{((xa,ta),(xb,tb)). xa = xb \<and> (\<exists>l. (l, Inl ta) \<in> set_bset (branches_sem_tree tb))}\<close>)
-   apply (clarsimp simp add: wf_def, rule sem_tree_induct, blast)
-  apply force
-  done
-
-function step_rel_sem_tree
-  :: \<open>('l \<Rightarrow> 's \<Rightarrow> 's + unit \<Rightarrow> bool) \<Rightarrow> ('c, 's, 'l) sem_tree \<Rightarrow> bool\<close>
-  where
-  \<open>step_rel_sem_tree r (Branch (s, c) S) =
-      pred_bset
-        (\<lambda>(l,mt'). r l s (map_sum (fst \<circ> config_sem_tree) id mt') \<and>
-                   (\<forall>t'. mt' = Inl t' \<longrightarrow> step_rel_sem_tree r t'))
-        S\<close>
-  by pat_completeness auto
-termination
-  apply (relation
-      \<open>{((xa,ta),(xb,tb)). xa = xb \<and> (\<exists>l. (l, Inl ta) \<in> set_bset (branches_sem_tree tb))}\<close>)
+      \<open>{((xa,ta),(xb,tb)).
+          xa = xb \<and> (\<exists>s l s'. (s, l, Inl (s', ta)) \<in> set_bset (branches_sem_tree tb))}\<close>)
    apply (clarsimp simp add: wf_def, rule sem_tree_induct, blast)
   apply force
   done
 
 
-function steps_pred_sem_tree
+
+
+definition config_pred_sem_tree :: \<open>('c \<Rightarrow> 's \<Rightarrow> bool) \<Rightarrow> ('c, 's, 'l) sem_tree \<Rightarrow> bool\<close> where
+  \<open>config_pred_sem_tree p t \<equiv>
+    pred_sem_tree (\<lambda>c S. \<forall>s l mst'. (s,l,mst') \<in> set_bset S \<longrightarrow> p c s) t\<close>
+
+definition precond_pred_sem_tree :: \<open>('s set \<Rightarrow> bool) \<Rightarrow> ('c, 's, 'l) sem_tree \<Rightarrow> bool\<close> where
+  \<open>precond_pred_sem_tree P t \<equiv> pred_sem_tree (\<lambda>_ S. P (fst ` set_bset S)) t\<close>
+
+definition step_rel_sem_tree :: \<open>('l \<Rightarrow> 's \<Rightarrow> 's + unit \<Rightarrow> bool) \<Rightarrow> ('c, 's, 'l) sem_tree \<Rightarrow> bool\<close>
+  where
+    \<open>step_rel_sem_tree r t =
+      pred_sem_tree (\<lambda>c S. \<forall>s l mst'. (s,l,mst') \<in> set_bset S \<longrightarrow> r l s (map_sum fst id mst')) t\<close>
+
+definition steps_pred_sem_tree
   :: \<open>(('s \<times> 'l \<times> ('s + unit)) set \<Rightarrow> bool) \<Rightarrow> ('c, 's, 'l) sem_tree \<Rightarrow> bool\<close>
   where
-  \<open>steps_pred_sem_tree p (Branch (s,c) S) =
-    (p (set_bset (map_bset (\<lambda>(l, mt'). (s, l, map_sum (fst \<circ> config_sem_tree) id mt')) S)) \<and>
-      pred_bset (\<lambda>v. \<forall>l t'. v = (l, Inl t') \<longrightarrow> steps_pred_sem_tree p t') S)\<close>
-  by pat_completeness auto
-termination
-  apply (relation
-      \<open>{((xa,ta),(xb,tb)). xa = xb \<and> (\<exists>l. (l, Inl ta) \<in> set_bset (branches_sem_tree tb))}\<close>)
-   apply (clarsimp simp add: wf_def, rule sem_tree_induct, blast)
-  apply force
-  done
+    \<open>steps_pred_sem_tree P t \<equiv>
+      pred_sem_tree
+        (\<lambda>_ S. P (set_bset (map_bset (\<lambda>(s, l, mst'). (s, l, map_sum fst id mst')) S)))
+        t\<close>
 
 (*
 definition
@@ -132,25 +143,34 @@ lemma sem_tree_contains_no_loop:
 
 fun bounded_treesem
   :: \<open>('s \<Rightarrow> 's \<Rightarrow> bool) \<Rightarrow>
-      ('l \<times> 's \<Rightarrow> bool) \<Rightarrow>
-      ('l::pre_perm_alg \<times> 's) \<times> ('l \<times> 's, unit) comm \<Rightarrow>
+      ('l::pre_perm_alg \<times> 's \<Rightarrow> bool) \<Rightarrow>
+      ('l \<times> 's, unit) comm \<Rightarrow>
+      'l \<times> 's \<Rightarrow>
       nat \<Rightarrow>
       (('l \<times> 's, unit) comm, 'l \<times> 's, unit label) sem_tree\<close>
   where
-  \<open>bounded_treesem r F sc 0 = Branch sc bempty\<close>
-| \<open>bounded_treesem r F (s, c) (Suc n) =
-    Branch (s, c)
-      (map_bset (apsnd
-        (\<lambda>(z', c').
-          case z' of
-            Inl s' \<Rightarrow> Inl (bounded_treesem r F (s', c') n)
-          | Inr () \<Rightarrow> Inr ()))
+  \<open>bounded_treesem r F c s 0 = Branch c bempty\<close>
+| \<open>bounded_treesem r F c (hl,hs) (Suc n) =
+    Branch c
+      (map_bset
+        (apsnd (apsnd (\<lambda>(z', c'). (map_sum (\<lambda>s'. (s', bounded_treesem r F c' s' n)) id z'))))
         (bCollect
-          (\<lambda>(l, (z', c')).
-              (\<exists>\<alpha>. l = Local \<alpha> \<and> (s, c) \<midarrow>\<alpha>\<rightarrow> (z', c')) \<or>
-              (\<exists>hs'. l = Env \<and> r (snd s) hs' \<and> z' = Inl (fst s, hs') \<and> c' = c))))\<close>
+          (\<lambda>((hlx,hsx), l, (z', c')).
+              hsx = hs \<and> (
+                (hlx = hl \<or> (\<exists>hlf. F (hlf, hsx) \<and> hl ## hlf \<and> hlx = hl + hlf)) \<and>
+                  (\<exists>\<alpha>. l = Local \<alpha> \<and> ((hlx,hsx), c) \<midarrow>\<alpha>\<rightarrow> (z', c')) \<or>
+                (hlx = hl \<and> c' = c \<and> (\<exists>hsx'. l = Env \<and> r hsx hsx' \<and> z' = Inl (hlx, hsx')))))))\<close>
 
-(* TODO: precondition limitations *)
+lemma precond_pred_sem_tree_mono:
+  \<open>p \<le> q \<Longrightarrow> pred_sem_tree p t \<Longrightarrow> pred_sem_tree q t\<close>
+  apply (induct t)
+  apply (clarsimp split: prod.splits)
+  apply (rule conjI, blast)
+  apply (rule bset.pred_mono_strong, assumption)
+  apply (clarsimp split: sum.splits)
+  done
+
+lemmas precond_pred_sem_tree_monoD = precond_pred_sem_tree_mono[rotated]
 
 (*
 definition treesem
@@ -164,29 +184,23 @@ definition treesem
 definition sem_tree_nocrash
   :: \<open>(('l \<times> 's, unit) comm, 'l \<times> 's, unit label) sem_tree \<Rightarrow> bool\<close>
   where
-  \<open>sem_tree_nocrash \<equiv> step_rel_sem_tree (\<lambda>_ _ z'. z' \<noteq> Inr ())\<close>
+    \<open>sem_tree_nocrash \<equiv> step_rel_sem_tree (\<lambda>_ _ z'. z' \<noteq> Inr ())\<close>
 
 definition sem_tree_post
-  :: \<open>('s \<Rightarrow> bool) \<Rightarrow>
-      (('s, unit) comm, 's, unit label) sem_tree \<Rightarrow>
-      bool\<close>
+  :: \<open>('s \<Rightarrow> bool) \<Rightarrow> (('s, unit) comm, 's, unit label) sem_tree \<Rightarrow> bool\<close>
   where
-  \<open>sem_tree_post q \<equiv> pred_sem_tree (\<lambda>(s,c). c = Skip \<longrightarrow> q s)\<close>
+    \<open>sem_tree_post q \<equiv> config_pred_sem_tree (\<lambda>c s. c = Skip \<longrightarrow> q s)\<close>
 
 definition sem_tree_guar
-  :: \<open>('s \<Rightarrow> 's \<Rightarrow> bool) \<Rightarrow>
-      (('l \<times> 's, unit) comm, 'l \<times> 's, unit label) sem_tree \<Rightarrow>
-      bool\<close>
+  :: \<open>('s \<Rightarrow> 's \<Rightarrow> bool) \<Rightarrow> (('l \<times> 's, unit) comm, 'l \<times> 's, unit label) sem_tree \<Rightarrow> bool\<close>
   where
-  \<open>sem_tree_guar g \<equiv>
-    step_rel_sem_tree (\<lambda>l s z'. \<forall>\<alpha> s'. l = Local \<alpha> \<longrightarrow> z' = Inl s' \<longrightarrow> g (snd s) (snd s'))\<close>
+    \<open>sem_tree_guar g \<equiv>
+      step_rel_sem_tree (\<lambda>l s z'. \<forall>\<alpha> s'. l = Local \<alpha> \<longrightarrow> z' = Inl s' \<longrightarrow> g (snd s) (snd s'))\<close>
 
 definition sem_tree_states
-  :: \<open>('l \<times> 's \<Rightarrow> bool) \<Rightarrow>
-      (('l \<times> 's, unit) comm, 'l \<times> 's, unit label) sem_tree \<Rightarrow>
-      bool\<close>
+  :: \<open>('l \<times> 's \<Rightarrow> bool) \<Rightarrow> (('l \<times> 's, unit) comm, 'l \<times> 's, unit label) sem_tree \<Rightarrow> bool\<close>
   where
-  \<open>sem_tree_states S \<equiv> pred_sem_tree (S \<circ> fst)\<close>
+    \<open>sem_tree_states S \<equiv> config_pred_sem_tree (\<lambda>_. S)\<close>
 
 definition sem_tree_frame_cond
   :: \<open>('l::pre_perm_alg \<times> 's \<Rightarrow> bool) \<Rightarrow>
@@ -221,7 +235,7 @@ definition sem_tree_safe
 lemma safe_then_sem_tree_safe:
   \<open>safe n c z r g q S F \<Longrightarrow>
     z = Inl s \<Longrightarrow>
-    sem_tree_safe q g S (bounded_treesem r F (s, c) n)\<close>
+    sem_tree_safe q g S (bounded_treesem r F c s n)\<close>
   apply (induct arbitrary: s rule: safe.inducts)
   sorry
 
